Cpc/Proofs/TypePreservation/Sets.lean
@@ -140,16 +140,18 @@ theorem mss_op_internal_typed
           simpa [__smtx_index_typeof_map] using congrArg __smtx_index_typeof_map hHead
         have hAccCons :
             __smtx_typeof_map_value
-                (__smtx_map_canon_insert e (SmtValue.Boolean true) acc) =
+                (__smtx_msm_update_aux (__smtx_msm_get_default acc) acc e
+                  (SmtValue.Boolean true)) =
               SmtType.Map A SmtType.Bool := by
           exact map_canon_insert_typed (m := acc) (A := A) (B := SmtType.Bool)
             hacc he rfl
         let acc' :=
           native_ite
-            (native_iff
-              (native_veq (__smtx_msm_lookup m2 e) (SmtValue.Boolean true))
-              isInter)
-            (__smtx_map_canon_insert e (SmtValue.Boolean true) acc) acc
+              (native_iff
+                (native_veq (__smtx_msm_lookup m2 e) (SmtValue.Boolean true))
+                isInter)
+            (__smtx_msm_update_aux (__smtx_msm_get_default acc) acc e
+              (SmtValue.Boolean true)) acc
         have hacc' : __smtx_typeof_map_value acc' = SmtType.Map A SmtType.Bool := by
           dsimp [acc']
           by_cases hKeep :
